theory/Bear/Graph.v
@@ -17,10 +17,30 @@ Record Graph : Type := {
   Vert_disc : Discrete Vert;
   Vert_enum : Enum Vert;
 
+  Vert_NoDup : NoDup enum;
+
   successors : Vert -> list Vert;
   }.
 
 Arguments successors {_} _.
+
+Lemma in_dec {X} `{Discrete X} (x : X) (xs : list X) :
+  { In x xs } + { ~ In x xs }.
+Proof.
+  induction xs as [|x' xs']; simpl.
+  - now right.
+  - destruct (eq_dec x' x).
+    + left; now left.
+    + destruct IHxs'.
+      * left; now right.
+      * right; intros [|]; contradiction.
+Defined.
+
+Definition in_decb {X} `{Discrete X} (x : X) (xs : list X) :=
+  match in_dec x xs with
+  | left _ => true
+  | right _ => false
+  end.
 
 Global Instance Graph_Vert_disc (G : Graph) : Discrete (Vert G) :=
   Vert_disc G.
@@ -28,18 +48,72 @@ Global Instance Graph_Vert_disc (G : Graph) : Discrete (Vert G) :=
 Global Instance Graph_Vert_enum (G : Graph) : Enum (Vert G) :=
   Vert_enum G.
 
-Fixpoint first_index_aux {X} `{Discrete X} n (x : X) xs : option nat :=
+Definition predecessors {G} (v : Vert G) : list (Vert G) :=
+  filter (fun v' =>
+    in_decb v (successors v')) enum.
+
+Lemma predecessors_correct_1 {G} (v v' : Vert G) :
+  In v' (successors v) -> In v (predecessors v').
+Proof.
+  intro pf.
+  unfold predecessors.
+  rewrite filter_In.
+  split; [apply enum_correct|].
+  unfold in_decb.
+  destruct in_dec; [reflexivity|contradiction].
+Qed.
+
+Lemma predecessors_correct_2 {G} (v v' : Vert G) :
+  In v (predecessors v') -> In v' (successors v).
+Proof.
+  intro pf.
+  unfold predecessors in pf.
+  rewrite filter_In in pf.
+  destruct pf as [_ pf].
+  unfold in_decb in pf.
+  destruct in_dec in pf; [auto|discriminate].
+Qed.
+
+Lemma predecessors_correct {G} (v v' : Vert G) :
+  In v' (successors v) <-> In v (predecessors v').
+Proof.
+  intros; split.
+  - apply predecessors_correct_1.
+  - apply predecessors_correct_2.
+Qed.
+
+Fixpoint first_index_aux {X} `{Discrete X} n xs (x : X) : option nat :=
   match xs with
   | [] => None
   | y :: ys =>
     match eq_dec x y with
     | left _ => Some n
-    | right _ => first_index_aux (S n) x ys
+    | right _ => first_index_aux (S n) ys x
     end
   end.
 
+Definition opt_le (o1 o2 : option nat) : Prop :=
+  match o1, o2 with
+  | None, _ => True
+  | Some x, None => False
+  | Some x, Some y => x <= y
+  end.
+
+(*
+Global Instance Ord_nat : Ord nat.
+Proof.
+  refine {|
+    ord_le := le
+  |}.
+  - apply PeanoNat.Nat.le_trans.
+  - intros x y; destruct (Compare_dec.le_dec x y).
+    + now left.
+    + right; lia.
+Defined.
+*)
+
 Lemma first_index_aux_bound {X} `{Discrete X} {xs} : forall {n x k},
-  first_index_aux n x xs = Some k -> n <= k.
+  first_index_aux n xs x = Some k -> n <= k.
 Proof.
   induction xs; intros n x k Hx.
   - now discriminate.
@@ -50,8 +124,8 @@ Proof.
 Defined.
 
 Lemma first_index_aux_inj {X} `{Discrete X} xs : forall n (x x' : X) k k',
-  first_index_aux n x xs = Some k ->
-  first_index_aux n x' xs = Some k' ->
+  first_index_aux n xs x = Some k ->
+  first_index_aux n xs x' = Some k' ->
   k = k' -> x = x'.
 Proof.
   induction xs; intros n x x' k k' Hx Hx' Hkk'.
@@ -67,7 +141,7 @@ Proof.
 Qed.
 
 Lemma first_index_aux_In {X} `{Discrete X} {xs} : forall n {x},
-  In x xs -> {k : nat & first_index_aux n x xs = Some k}.
+  In x xs -> { k : nat & first_index_aux n xs x = Some k }.
 Proof.
   induction xs; intros n x HIn.
   - destruct HIn.
@@ -78,9 +152,12 @@ Proof.
       destruct HIn; [congruence|auto].
 Defined.
 
+(*
 Definition inj_nat {X} `{Discrete X} `{Enum X} : X -> nat :=
   fun x => projT1 (first_index_aux_In 0 (enum_correct x)).
+*)
 
+(*
 Lemma inj_nat_correct {X} `{Discrete X} `{Enum X} :
   forall (x x' : X), inj_nat x = inj_nat x' -> x = x'.
 Proof.
@@ -91,17 +168,129 @@ Proof.
   simpl in Hxx'; subst.
   eapply first_index_aux_inj; eauto.
 Qed.
+*)
 
 Global Instance subcount_Ord {X} `{Discrete X, Enum X} : Ord X.
 Proof.
   refine {|
-    ord_le := fun x y => inj_nat x <= inj_nat y;
+    ord_le := fun x y => opt_le (first_index_aux 0 enum x) (first_index_aux 0 enum y);
     ord_le_trans := _;
     ord_le_dec := _
   |}.
-  - intros; eapply PeanoNat.Nat.le_trans; eauto.
-  - intros.
-    destruct (Compare_dec.le_le_S_dec (inj_nat x) (inj_nat y)).
+  - intros x y z Hxy Hyz.
+    unfold opt_le in *.
+    destruct (first_index_aux_In 0 (enum_correct x)) as [a Ha].
+    destruct (first_index_aux_In 0 (enum_correct y)) as [b Hb].
+    destruct (first_index_aux_In 0 (enum_correct z)) as [c Hc].
+    rewrite Ha, Hb, Hc in *.
+    now apply (PeanoNat.Nat.le_trans _ b).
+  - intros x y.
+    unfold opt_le.
+    destruct (first_index_aux_In 0 (enum_correct x)) as [a Ha].
+    destruct (first_index_aux_In 0 (enum_correct y)) as [b Hb].
+    rewrite Ha, Hb.
+    destruct (Compare_dec.le_le_S_dec a b).
     + now left.
     + right; lia.
+  - intros x y.
+    unfold opt_le.
+    destruct (first_index_aux_In 0 (enum_correct x)) as [a Ha].
+    destruct (first_index_aux_In 0 (enum_correct y)) as [b Hb].
+    rewrite Ha, Hb.
+    intros.
+    eapply first_index_aux_inj; eauto.
+    lia.
 Defined.
+
+Lemma Forall_map_lemma {X Y} (f : X -> Y) (P : Y -> Prop) : forall xs,
+  Forall P (map f xs) -> Forall (fun x => P (f x)) xs.
+Proof.
+  induction xs as [|x xs']; intro HP.
+  - constructor.
+  - inversion HP; constructor; auto.
+Qed.
+
+Lemma sort_map_lemma {X Y} (f : X -> Y) (R : Y -> Y -> Prop) :
+  forall xs, Sorted.StronglySorted R (map f xs) ->
+  Sorted.StronglySorted (fun x y => R (f x) (f y)) xs.
+Proof.
+  induction xs; intros HR.
+  - constructor.
+  - inversion HR.
+    constructor.
+    + now apply IHxs.
+    + now apply Forall_map_lemma.
+Qed.
+
+Lemma map_ext_lemma {X Y} (f g : X -> Y) :
+  forall xs, (forall x, In x xs -> f x = g x) ->
+  map f xs = map g xs.
+Proof.
+  induction xs; intro Hfg.
+  - reflexivity.
+  - simpl.
+    rewrite Hfg; [|now left].
+    rewrite IHxs; [reflexivity|].
+    intros x Hx.
+    apply Hfg; now right.
+Qed.
+
+Lemma first_index_aux_NoDup_bound {X} `{Discrete X} : forall (xs : list X),
+  NoDup xs -> forall m n, m <= n ->
+  Forall (opt_le (Some m)) (map (first_index_aux n xs) xs).
+Proof.
+  induction xs as [|x xs']; intros pf m n Hmn.
+  - constructor.
+  - simpl; constructor.
+    + simpl; destruct (eq_dec x x); [lia|contradiction].
+    + simpl.
+      assert (
+        map (fun y =>
+          if eq_dec y x then Some n else first_index_aux (S n) xs' y) xs' =
+        map (first_index_aux (S n) xs') xs') as eq_pf.
+      { apply map_ext_lemma.
+        intros y Hy.
+        destruct (eq_dec y x); [|reflexivity].
+        inversion pf; congruence.
+      }
+      rewrite eq_pf.
+      apply IHxs'; [|lia].
+      now inversion pf.
+Qed.
+
+Lemma first_index_aux_NoDup_sorted {X} `{Discrete X}
+  : forall (xs : list X), NoDup xs -> forall n,
+  Sorted.StronglySorted opt_le (map (first_index_aux n xs) xs).
+Proof.
+  induction xs; intros.
+  - constructor.
+  - simpl.
+    destruct (eq_dec a a); [|contradiction].
+    assert (
+      map (fun x =>
+        if eq_dec x a then Some n else first_index_aux (S n) xs x) xs =
+      map (first_index_aux (S n) xs) xs) as pf.
+    { apply map_ext_lemma.
+      intros x Hx.
+      destruct (eq_dec x a); [|reflexivity].
+      inversion H0.
+      congruence.
+    }
+    rewrite pf.
+    constructor.
+    + apply IHxs.
+      now inversion H0.
+    + apply first_index_aux_NoDup_bound; [|lia].
+      now inversion H0.
+Qed.
+
+Lemma enum_sorted {X} `{Discrete X, Enum X} :
+  NoDup enum -> sorted (enum : list X).
+Proof.
+  unfold sorted.
+  unfold ord_le.
+  unfold subcount_Ord.
+  intro.
+  apply sort_map_lemma.
+  now apply first_index_aux_NoDup_sorted.
+Qed.
