theory/Bear/Sort.v
@@ -5,7 +5,8 @@ Require Import Sorting.
 Class Ord (X : Type) := {
   ord_le : X -> X -> Prop;
   ord_le_trans : forall x y z, ord_le x y -> ord_le y z -> ord_le x z;
-  ord_le_dec : forall x y, { ord_le x y } + { ord_le y x }
+  ord_le_dec : forall x y, { ord_le x y } + { ord_le y x };
+  ord_le_antisym : forall x y, ord_le x y -> ord_le y x -> x = y
   }.
 
 Definition sorted {X} `{Ord X} : list X -> Prop :=
@@ -77,20 +78,110 @@ Proof.
   - now apply insert_sorted.
 Qed.
 
+Lemma insert_length {X} `{Ord X} (x : X) (xs : list X) :
+  length (insert x xs) = S (length xs).
+Proof.
+  induction xs.
+  - reflexivity.
+  - simpl.
+    destruct (ord_le_dec x a).
+    + reflexivity.
+    + simpl; congruence.
+Qed.
+
 Lemma insertion_sort_length {X} `{Ord X} (xs : list X) :
   length (insertion_sort xs) = length xs.
 Proof.
-Admitted.
+  induction xs; intros.
+  - reflexivity.
+  - simpl.
+    rewrite insert_length; congruence.
+Qed.
 
-Lemma insertion_sort_NoDup {X} `{Ord X} (xs : list X) :
-  NoDup xs -> NoDup (insertion_sort xs).
+Lemma insert_In_1 {X} `{Ord X} (x : X) (xs : list X) :
+  forall y, In y (insert x xs) -> (x = y \/ In y xs).
 Proof.
-Admitted.
+  induction xs; intros y Hy.
+  - left; now destruct Hy.
+  - simpl in Hy.
+    destruct (ord_le_dec x a).
+    + destruct Hy; auto.
+    + simpl in *; firstorder.
+Qed.
+
+Lemma insert_In_2 {X} `{Ord X} (x : X) (xs : list X) :
+  forall y, (x = y \/ In y xs) -> In y (insert x xs).
+Proof.
+  induction xs; intros y Hy.
+  - simpl in *; tauto.
+  - simpl.
+    destruct (ord_le_dec x a); simpl in *; firstorder.
+Qed.
+
+Lemma insert_In {X} `{Ord X} (x : X) (xs : list X) :
+  forall y, In y (insert x xs) <-> (x = y \/ In y xs).
+Proof.
+  intro; split.
+  - apply insert_In_1.
+  - apply insert_In_2.
+Qed.
+
+Lemma insertion_sort_In_1 {X} `{Ord X} (xs : list X) :
+  forall x, In x (insertion_sort xs) -> In x xs.
+Proof.
+  induction xs; intros x Hx.
+  - destruct Hx.
+  - simpl in Hx.
+    rewrite insert_In in Hx.
+    simpl; firstorder.
+Qed.
+
+Lemma insertion_sort_In_2 {X} `{Ord X} (xs : list X) :
+  forall x, In x xs -> In x (insertion_sort xs).
+Proof.
+  induction xs; intros x Hx.
+  - destruct Hx.
+  - simpl.
+    rewrite insert_In.
+    simpl in Hx; firstorder.
+Qed.
 
 Lemma insertion_sort_In {X} `{Ord X} (xs : list X) :
   forall x, In x (insertion_sort xs) <-> In x xs.
 Proof.
-Admitted.
+  intro; split.
+  - apply insertion_sort_In_1.
+  - apply insertion_sort_In_2.
+Qed.
+
+Lemma insert_NoDup {X} `{Ord X} (x : X) xs :
+  NoDup xs -> ~ In x xs -> NoDup (insert x xs).
+Proof.
+  induction xs; intros nd nIn.
+  - constructor; auto.
+  - simpl.
+    destruct (ord_le_dec x a).
+    + now constructor.
+    + constructor.
+      * rewrite insert_In.
+        intros [pf|pf].
+        -- simpl in nIn; auto.
+        -- now inversion nd.
+      * apply IHxs.
+        -- now inversion nd.
+        -- simpl in nIn; auto.
+Qed.
+
+Lemma insertion_sort_NoDup {X} `{Ord X} (xs : list X) :
+  NoDup xs -> NoDup (insertion_sort xs).
+Proof.
+  induction xs; intro pf.
+  - constructor.
+  - simpl.
+    inversion pf.
+    apply insert_NoDup; auto.
+    now rewrite insertion_sort_In.
+Qed.
 
 Fixpoint sublists {X} n (xs : list X) {struct xs} : list (list X) :=
   match n with
@@ -102,3 +193,177 @@ Fixpoint sublists {X} n (xs : list X) {struct xs} : list (list X) :=
     end
   end.
 
+Lemma sublist_length {X} (xs : list X) : forall n ys,
+  In ys (sublists n xs) -> length ys = n.
+Proof.
+  induction xs; intros n ys Hys.
+  - destruct ys; simpl in Hys.
+    + destruct n; [reflexivity|destruct Hys].
+    + destruct n; now inversion Hys.
+  - simpl in Hys.
+    destruct n.
+    + inversion Hys as [H|H];
+      now destruct H.
+    + rewrite in_app_iff in Hys.
+      destruct Hys as [H|H].
+      * rewrite in_map_iff in H.
+        destruct H as [l [Hl1 Hl2]].
+        rewrite <- Hl1; simpl.
+        now rewrite (IHxs _ _ Hl2).
+      * now apply IHxs.
+Qed.
+
+Lemma sublist_In_trans {X} (xs : list X)
+  : forall n x ys, In x ys -> In ys (sublists n xs) -> In x xs.
+Proof.
+  induction xs; intros n x ys Hx Hys.
+  - simpl in Hys.
+    destruct n.
+    + destruct Hys as [H|H].
+      * congruence.
+      * destruct H.
+    + destruct Hys.
+  - simpl in Hys.
+    destruct n.
+    + destruct Hys as [H|H].
+      * rewrite <- H in Hx; destruct Hx.
+      * destruct H.
+    + rewrite in_app_iff in Hys.
+      destruct Hys.
+      * rewrite in_map_iff in H.
+        destruct H as [l [Hl1 Hl2]].
+        rewrite <- Hl1 in Hx.
+        destruct Hx.
+        -- now left.
+        -- right; eapply IHxs; eauto.
+      * right; eapply IHxs; eauto.
+Qed.
+
+Lemma sublist_Forall {X} (xs : list X) (P : X -> Prop)
+  : Forall P xs -> forall n ys, In ys (sublists n xs) ->
+    Forall P ys.
+Proof.
+  induction xs; intros Hxs n ys Hys.
+  - destruct n; simpl in Hys.
+    + destruct Hys as [[]|[]].
+      constructor.
+    + destruct Hys.
+  - destruct n; simpl in Hys.
+    + destruct Hys as [[]|[]].
+      constructor.
+    + rewrite in_app_iff in Hys.
+      destruct Hys as [pf|pf].
+      * rewrite in_map_iff in pf.
+        destruct pf as [l [[] Hl2]].
+        inversion Hxs; constructor; auto.
+        eapply IHxs; eauto.
+      * eapply IHxs; eauto.
+        now inversion Hxs.
+Qed.
+
+Lemma sublist_sort {X} `{Ord X} (xs : list X) :
+  forall n ys, In ys (sublists n xs) ->
+  sorted xs -> sorted ys.
+Proof.
+  unfold sorted.
+  induction xs; intros n ys Hys xs_sort.
+  - destruct n; simpl in Hys.
+    + destruct Hys as [pf|[]].
+      rewrite <- pf.
+      constructor.
+    + destruct Hys.
+  - destruct n; simpl in Hys.
+    + destruct Hys as [pf|[]].
+      rewrite <- pf.
+      constructor.
+    + rewrite in_app_iff in Hys.
+      destruct Hys as [pf|pf].
+      * rewrite in_map_iff in pf.
+        destruct pf as [l [Hl1 Hl2]].
+        rewrite <- Hl1.
+        inversion xs_sort.
+        constructor.
+        -- eapply IHxs; eauto.
+        -- eapply sublist_Forall; eauto.
+      * inversion xs_sort.
+        eapply IHxs; eauto.
+Qed.
+
+Lemma filter_Forall {X} (xs : list X)
+  (P : X -> Prop) (p : X -> bool) :
+  Forall P xs -> Forall P (filter p xs).
+Proof.
+  induction xs; intros Hxs.
+  - constructor.
+  - inversion Hxs.
+    simpl; destruct (p a).
+    + constructor; auto.
+    + now apply IHxs.
+Qed.
+
+Lemma sorted_filter {X} `{Ord X} (p : X -> bool) (xs : list X) :
+  sorted xs -> sorted (filter p xs).
+Proof.
+  induction xs; intros xs_sort.
+  - constructor.
+  - simpl.
+    inversion xs_sort.
+    destruct (p a).
+    + constructor.
+      * now apply IHxs.
+      * now apply filter_Forall.
+    + now apply IHxs.
+Qed.
+
+Lemma in_sublists {X} `{Ord X} :
+  forall xs, NoDup xs -> sorted xs ->
+  forall ys, NoDup ys -> sorted ys ->
+  (forall y, In y ys -> In y xs) ->
+  forall n, length ys = n ->
+  In ys (sublists n xs).
+Proof.
+  induction xs; intros nd_xs sort_xs ys nd_ys sort_ys ys_sublist n ys_len.
+  - simpl; destruct n.
+    + destruct ys; [now left|].
+      discriminate.
+    + destruct ys; [discriminate|].
+      elim (ys_sublist x).
+      now left.
+  - simpl; destruct n.
+    + destruct ys; [now left|].
+      discriminate.
+    + rewrite in_app_iff.
+      destruct ys as [|y zs]; [discriminate|].
+      destruct (ys_sublist y) as [pf|pf]; [now left| |].
+      * left.
+        rewrite <- pf.
+        apply in_map.
+        apply IHxs.
+        -- now inversion nd_xs.
+        -- now inversion sort_xs.
+        -- now inversion nd_ys.
+        -- now inversion sort_ys.
+        -- intros z Hz.
+           destruct (ys_sublist z); [now right| |auto].
+           inversion nd_ys; congruence.
+        -- simpl in ys_len; congruence.
+      * right.
+        apply IHxs.
+        -- now inversion nd_xs.
+        -- now inversion sort_xs.
+        -- now inversion nd_ys.
+        -- now inversion sort_ys.
+        -- intros z [Heq|HIn]; [now rewrite <- Heq|].
+           destruct (ys_sublist z) as [pf'|]; [now right| |auto].
+           absurd (y = z).
+           ++ inversion nd_ys; congruence.
+           ++ apply ord_le_antisym.
+              ** inversion sort_ys as [|? ? ? Hy].
+                 rewrite Forall_forall in Hy.
+                 now apply Hy.
+              ** rewrite pf' in *.
+                 inversion sort_xs as [|? ? ? Hz].
+                 rewrite Forall_forall in Hz.
+                 now apply Hz.
+        -- auto.
+Qed.
